Add broadcasting and strides
This also adds NonEmptyList as a new type for shapes, since shapes
can't be empty.

TensorLib/NumpyRepr.lean
@@ -1,16 +1,21 @@
 import Init.System.IO
 import Init.System.FilePath
 import Mathlib.Tactic
+import TensorLib.NonEmptyList
 import TensorLib.TensorElement
 
-/-
-https://numpy.org/doc/stable/reference/generated/numpy.lib.format.html
-https://github.com/numpy/numpy/blob/067cb067cb17a20422e51da908920a4fbb3ab851/doc/neps/nep-0001-npy-format.rst
+/-!
+We largely duplicate the NumPy representation of tensors.
+
+The binary format is described here: https://numpy.org/doc/stable/reference/generated/numpy.lib.format.html
+and here: https://github.com/numpy/numpy/blob/067cb067cb17a20422e51da908920a4fbb3ab851/doc/neps/nep-0001-npy-format.rst
+
+In addition to being efficient, this allows us to directly parse .npy input files.
 -/
 
 namespace TensorLib
 
--- The subset of types NumPy supports that we care about
+/-! The subset of types NumPy supports that we care about -/
 inductive NumpyDtype where
 | bool
 | int8
@@ -28,14 +33,22 @@ inductive NumpyDtype where
 
 namespace NumpyDtype
 
+--! Number of bytes used by each element of the given dtype
 def bytes (x: NumpyDtype): Nat := match x with
 | float64 | int64 | uint64 => 8
 | float32 | int32 | uint32 => 4
 | float16 | int16 | uint16 => 2
 | bool | int8 | uint8 => 1
 
--- Disk formats found through experimentation. Not sure why there are
--- both '<' and '|' as prefixes
+/-!
+Parse a numpy dtype.
+
+Disk formats found through experimentation. Not sure why there are
+both '<' and '|' as prefixes. The first character represents the
+byte order: https://numpy.org/doc/2.1/reference/generated/numpy.dtype.byteorder.html
+'<' is little endian, '|' is "not applicable" Not sure why bool showed up
+as both.
+-/
 def fromString (s: String) : Except String NumpyDtype := match s with
 | "<b1" | "|b1"=> .ok bool
 | "|i1" => .ok int8
@@ -53,24 +66,98 @@ def fromString (s: String) : Except String NumpyDtype := match s with
 
 end NumpyDtype
 
+--! Numpy disk format uses python convention for bools; True/False
 def NumpyBool.fromString (s: String): Except String Bool := match s with
 | "True" => .ok true
 | "False" => .ok false
 | _ => .error s!"Can't parse {s} as Bool"
 
-abbrev Shape := List Nat
+/-!
+Shapes and strides in tensors are represented as lists, where the length of the
+list is the number of dimensions. For example, a 2 x 3 matrix has a shape of [2, 3].
+
+```
+>>> x = np.arange(6).reshape(2, 3)
+>>> x
+array([[0, 1, 2],
+       [3, 4, 5]])
+>>> x.shape
+(2, 3)
+```
+
+(See https://web.mit.edu/dvp/Public/numpybook.pdf for extensive discussion of shape and stride.)
+
+What about the unit element? What is the shape of an empty tensor? For example,
+what is the shape of the 1D empty array `[]`? We follow NumPy by defining the shape
+as a 1d matrix with 0 elements.
+
+```
+>>> np.array([]).shape
+(0,)
+```
+
+(Assuming we allow 0s in other dimensions, we can shape-check the empty tensor at other shapes, e.g.
+`np.array([]).reshape([1,2,3,0,5])` succeeds.)
+
+The only way to have an empty shape in Numpy is as
+
+```
+>>> np.array(None).shape
+()
+```
+
+We can't write None in Lean, nor do we want to. If we allow empty lists in shape computation, we
+will need to continually handle the [] case with something like
+
+```
+match shape with
+| [] => impossible
+| x :: xs => E(x, xs)
+```
+
+As a result, we would either be in an error monad constantly for  no reason, or need to pass
+non-emptiness proofs around. For now, we avoid this case using NonemptyList.
+-/
+abbrev Shape := NonEmptyList Nat
+abbrev Strides := NonEmptyList Nat
 
 namespace Shape
 
-def count (s: Shape): Nat := match s with
-| [] => 0
-| [x] => x
-| x :: xs => x * count xs
+--! The number of elements in a tensor. All that's needed is the shape for this calculation.
+def count (s : Shape) : Nat := match s with
+| .mk x xs => xs.foldl (fun x y => x * y) x
 
--- def parse (s: String)
+/-!
+Strides can be computed from the shape by figuring out how many elements you
+need to jump over to get to the next spot and mulitplying by the bytes in each
+element.
+
+A given shape can have different strides if the tensor is a view of another
+tensor. For example, in a square matrix, the transposed matrix view has the same
+shape but the strides change.
+-/
+def defaultStrides (dtype : NumpyDtype) (s : Shape) : Strides :=
+  let s := s.reverse
+  let bytes := dtype.bytes
+  let rec loop (xs : List ℕ) (lastShape lastDimSize : ℕ): List ℕ := match xs with
+  | [] => []
+  | d :: ds =>
+    let rest := loop ds (lastShape * lastDimSize) d
+    lastShape * lastDimSize :: rest
+  let res : Strides := { hd := dtype.bytes, tl := loop s.tl bytes s.hd }
+  res.reverse
+
+#eval defaultStrides NumpyDtype.uint32 [2]
+#eval defaultStrides NumpyDtype.uint32 [2, 3]
+#eval defaultStrides NumpyDtype.uint32 [2, 3, 5, 7]
 
 end Shape
 
+/-!
+This is the header of the on-disk Numpy format, typically with the .npy file extension.
+
+https://numpy.org/doc/stable/reference/generated/numpy.lib.format.html#format-version-1-0
+-/
 structure NumpyHeader where
   -- Version is major.minor
   major : Nat
@@ -88,28 +175,167 @@ structure NumpyHeader where
 
 namespace NumpyHeader
 
+/-!
+A npy binary file has a header, some padding, then the data. This method computes the
+size of the data portion of the file.
+-/
 def dataSize (header : NumpyHeader): Nat := header.descr.bytes * header.shape.count
 
 end NumpyHeader
 
+-- We generally have huge tensors, so don't show them by default
 instance ByteArrayRepr : Repr ByteArray where
   reprPrec x _ :=
     let s := toString x.size
     s!"ByteArray of size {s}"
 
+/-!
+A NumpyRepr is the data of the tensor, along with all metadata required to do
+efficient computation. The `startIndex`, `endIndex`, and `strides` are inferred
+from parsing or computed during a view creation.
+-/
 structure NumpyRepr where
   header : NumpyHeader
   data : ByteArray
-  startIndex : Nat -- Pointer to the first byte of ndarray data
+  startIndex : Nat -- Pointer to the first byte of ndarray data, called `offset` in numpy
   endIndex : Nat   -- Pointer to the byte after the last byte of ndarray data
   -- invariant: startIndex <= endIndex
   -- invariant: endIndex - startIndex = descr.bytes * shape.count
   -- invariant: header.endIndex <= |data|
   -- invariant: header.dataSize <= |data|
+  strides : Strides
   deriving Repr
 
 namespace NumpyRepr
 
+--! shape
+def shape (x : NumpyRepr) : Shape := x.header.shape
+
+--! number of dimensions
+def ndim (x : NumpyRepr) : ℕ := x.shape.length
+
+--! number of elements
+def size (x : NumpyRepr) : ℕ := x.shape.count
+
+--! number of bytes representing each element
+def itemsize (x : NumpyRepr) : ℕ := x.header.descr.bytes
+
+--! number of bytes representing the entire tensor
+def nbytes (x : NumpyRepr) : ℕ := x.itemsize * x.size
+
+section Shape
+
+abbrev M a := Except String a
+
+/-!
+Reshaping a tensor is just re-interpreting the elements in
+a different order. This will also impact the iteration order/strides
+when we implement those.
+-/
+def reshape (x : NumpyRepr) (shape : Shape) : M NumpyRepr := do
+  if x.shape.count == shape.count then
+    return { x with header.shape := shape }
+  else
+    .error "Reshaping must have the same number of implied elements"
+
+end Shape
+
+/-!
+Broadcasting is a convenience and performance trick to allow operations that expect the same
+shaped arguments to work on non-matching arguments.  For example, we would like to be able
+to add 1 to each element of a tensor without building the all-1s tensor in memory.
+It involves applying the following rules to two tensors
+
+1. If the shape of one is smaller than the other, pad the smaller one
+   with 1s until they are the same length
+2. For each pair of numbers at each index, to broadcast either the
+   numbers must be the same, or one of them should be 1. In the later
+   case we replace that shape with the other number
+
+For example, we broadcast (3, 2, 1) (2, 7) to (3, 2, 7).
+
+A: (3, 2, 1)
+B: (2, 7)
+
+Rule 1
+
+A: (3, 2, 1)
+B: (1, 2, 7)
+
+Rule 2
+
+A: (3, 2, 1)
+B: (3, 2, 7)
+
+Rule 2
+
+A: (3, 2, 7)
+B: (3, 2, 7)
+-/
+structure Broadcast where
+  left : Shape
+  right : Shape
+  deriving BEq, Repr
+
+section Broadcast
+
+-- In broadcasting, we first extend the shorter array by prefixing 1s.
+-- NKI semantics currently suffixes 1s in some cases, so be explicit about
+-- the naming.
+private def oneExtendPrefix (b : Broadcast) : Broadcast :=
+  let n1 := b.left.length
+  let n2 := b.right.length
+  if n1 <= n2
+  then { b with left := .appendListL (List.replicate (n2 - n1) 1) b.left }
+  else { b with right := .appendListL (List.replicate (n1 - n2) 1) b.right }
+
+private theorem oneExtendPrefixLength (b : Broadcast) :
+  let b' := oneExtendPrefix b
+  b'.left.length = b'.right.length := by
+  cases b
+  rename_i left right
+  simp [oneExtendPrefix]
+  by_cases H : left.length <= right.length
+  . simp [H]
+    rw [NonEmptyList.appendListLLength, List.length_replicate, Nat.sub_add_cancel]
+    exact H
+  . simp [H]
+    rw [NonEmptyList.hAppendListLLength, List.length_replicate, Nat.sub_add_cancel]
+    linarith
+
+private def matchPairs (b : Broadcast) : Option Shape :=
+  if b.left.length != b.right.length then none else
+  let f xy := match xy with
+    | (x, y) =>
+      if x == y then some x
+      else if x == 1 then some y
+      else if y == 1 then some x
+      else none
+  traverse f (NonEmptyList.zip b.left b.right)
+
+--! Returns the shape resulting from broadcast the arguments
+def broadcast (b : Broadcast) : Option Shape := matchPairs (oneExtendPrefix b)
+
+--! Whether broadcasting is possible
+def canBroadcast (b : Broadcast) : Bool := (broadcast b).isSome
+
+#eval matchPairs (Broadcast.mk [1, 2, 3] [7, 2, 1])
+#eval broadcast (Broadcast.mk [1, 2, 3] [7, 7, 9, 2, 1])
+
+-- todo: add plausible properties when property-based testing settles down in Lean-land
+#guard
+ let x1 := [1,2,3]
+ let x2 := [2,3]
+ let b1 := Broadcast.mk x1 x1
+ let b2 := Broadcast.mk x1 x2
+ oneExtendPrefix b1 == b1 &&
+ broadcast b2 == broadcast b1 &&
+ broadcast b2 == some (.fromList! [1, 2, 3])
+
+end Broadcast
+
+
+--! Parse a .npy file
 namespace Parse
 
 structure ParsingState where
@@ -122,7 +348,17 @@ structure ParsingState where
   debug : List String
   deriving Repr
 
-abbrev PState (T : Type) := StateT ParsingState (Except String) T
+abbrev PState (T : Type) := EStateM String ParsingState T
+
+instance : MonadLiftT (Except String) PState where
+  monadLift x := match x with
+  | .ok x => .ok x
+  | .error x => .error x
+
+-- Except is nicer sometimes
+def resultExcept {σ : Type} (x : EStateM.Result String σ a) : Except String a := match x with
+| .ok x _ => .ok x
+| .error x _ => .error x
 
 variable {T : Type}
 
@@ -145,8 +381,8 @@ def whitespace : PState Unit := do
 
 def tryParse (p : PState T) : PState (Option T) := fun s =>
   match p s with
-  | .error _ => .ok (none, s)
-  | .ok (x, s) => .ok (some x, s)
+  | .error _ s => .ok none s
+  | .ok x s => .ok (some x) s
 
 def ignore (p : PState T) : PState Unit := do
   let _ <- tryParse p
@@ -203,9 +439,9 @@ def parseCommaList {T : Type} (start : Char) (end_ : Char) (p : PState T) : PSta
   consume end_
   return xs
 
-def parseShape : PState Shape := do
+partial def parseShape : PState Shape := do
   let xs <- parseCommaList '(' ')' parseToken
-  return xs.map (fun x => x.toNat!)
+  return .fromList! (xs.map (fun x => x.toNat!))
 
 -- major/minor/header-length
 def parseHeader : PState (Nat × Nat) := do
@@ -237,7 +473,7 @@ def parseOneMetadata : PState Unit := do
     modify (fun s => { s with descr := some d })
   else if id == "fortran_order" then
     let v <- parseToken
-    let b <- NumpyBool.fromString v
+    let b <- liftM (NumpyBool.fromString v)
     modify (fun s => { s with fortranOrder := b })
   else if id == "shape" then
     let shape <- parseShape
@@ -263,12 +499,14 @@ def parseNumpyRepr : PState NumpyRepr := do
   match s.descr, s.fortranOrder, s.shape with
   | some descr, some fortranOrder, some shape =>
     let numpyHeader := NumpyHeader.mk major minor descr fortranOrder shape
-    let repr := NumpyRepr.mk numpyHeader s.source s.headerEnd s.source.size
+    let strides := shape.defaultStrides descr
+    let repr := NumpyRepr.mk numpyHeader s.source s.headerEnd s.source.size strides
     return repr
   | _, _, _ => .error "Can't parse a metadata value"
 
 def parse (buffer : ByteArray) : Except String NumpyRepr := do
-  parseNumpyRepr.eval <| ParsingState.mk buffer 0 0 none none none []
+  let init := ParsingState.mk buffer 0 0 none none none []
+  resultExcept $ parseNumpyRepr.run init
 
 def parseFile (path: System.FilePath) : IO (Except String NumpyRepr) := do
   let buffer <- IO.FS.readBinFile path
