TensorLib/NonEmptyList.lean
@@ -1,0 +1,126 @@
+/-
+Copyright (c) 2024 Amazon.com, Inc. or its affiliates. All Rights Reserved.
+Released under Apache 2.0 license as described in the file LICENSE.
+Authors: Jean-Baptiste Tristan, Paul Govereau, Sean McLaughlin
+-/
+
+import Mathlib.Tactic
+
+/-!
+# Nonempty lists
+-/
+namespace TensorLib
+
+variable {a: Type}
+
+structure NonEmptyList (a: Type) where
+  hd: a
+  tl: List a
+  deriving BEq, Inhabited
+
+namespace NonEmptyList
+
+def toList (x: NonEmptyList a): List a := x.hd :: x.tl
+
+instance : Coe (NonEmptyList α) (List α) where
+  coe := toList
+
+instance : CoeDep (List α) (x :: xs) (NonEmptyList α) where
+  coe := { hd := x, tl := xs }
+
+-- Use the nice list bracket concrete syntax
+instance NelRepr [Repr a] : Repr (NonEmptyList a) where
+  reprPrec x n := reprPrec x.toList n
+
+def length (x: NonEmptyList a): Nat := 1 + x.tl.length
+
+@[simp]
+def append (x : NonEmptyList a) (y : NonEmptyList a) : NonEmptyList a :=
+  NonEmptyList.mk x.hd (x.tl ++ y.toList)
+
+theorem appendLength (x y : NonEmptyList a) : (append x y).length = x.length + y.length := by
+  simp [length, toList]
+  linarith
+
+instance : HAppend (NonEmptyList a) (NonEmptyList a) (NonEmptyList a) where
+  hAppend := append
+
+theorem hAppendLength (x y : NonEmptyList a) : (x ++ y).length = x.length + y.length := by
+  apply appendLength
+
+def appendListL (x : List a) (y : NonEmptyList a) := match x with
+| [] => y
+| x :: xs => NonEmptyList.mk x (xs ++ y.toList)
+
+theorem appendListLLength (x : List a) (y : NonEmptyList a) : (appendListL x y).length = x.length + y.length := by
+  induction x
+  . simp [appendListL]
+  . simp [appendListL, NonEmptyList.length, NonEmptyList.toList]
+    linarith
+
+instance HAppendListL : HAppend (List a) (NonEmptyList a) (NonEmptyList a) where
+  hAppend := appendListL
+
+theorem hAppendListLLength (x : List a) (y : NonEmptyList a) : (appendListL x y).length = x.length + y.length := by
+  apply appendListLLength
+
+def appendListR (x : NonEmptyList a) (y : List a) := NonEmptyList.mk x.hd (x.tl ++ y)
+
+instance HAppendListR : HAppend (NonEmptyList a) (List a) (NonEmptyList a) where
+  hAppend := appendListR
+
+theorem appendListRLength (x : NonEmptyList a) (y : List a) : (appendListR x y).length = x.length + y.length := by
+  simp [appendListR, NonEmptyList.length]
+  linarith
+
+theorem hAppendListRLength (x : NonEmptyList a) (y : List a) : (appendListR x y).length = x.length + y.length := by
+  apply appendListRLength
+
+def all (x: NonEmptyList a) (P: a -> Bool): Bool :=
+  P x.hd && x.tl.all P
+
+def contains [BEq a] (x : NonEmptyList a) (y : a) : Bool := (y == x.hd) || x.tl.contains y
+
+def map {b : Type} (f : a -> b) (x : NonEmptyList a) : NonEmptyList b :=
+  NonEmptyList.mk (f x.hd) (List.map f x.tl)
+
+def zipWith {b c : Type} (f : a -> b -> c) (x : NonEmptyList a) (y : NonEmptyList b) : NonEmptyList c :=
+  NonEmptyList.mk (f x.hd y.hd) (List.zipWith f x.tl y.tl)
+
+def zip {b : Type} (x : NonEmptyList a) (y : NonEmptyList b) : NonEmptyList (a × b) :=
+  zipWith (fun x y => (x, y)) x y
+
+def foldl {b : Type} (f : a -> b -> a) (x : a) (xs : NonEmptyList b) : a :=
+  List.foldl f (f x xs.hd) xs.tl
+
+def foldr {b : Type} (f : a -> b -> b) (x : b) (xs : NonEmptyList a) : b :=
+  List.foldr f (f xs.hd x) xs.tl
+
+def traverse [Applicative F] (f : α → F β) (x: NonEmptyList α) : F (NonEmptyList β) :=
+   NonEmptyList.mk <$> f x.hd <*> List.traverse f x.tl
+
+def reverse (x : NonEmptyList a) : NonEmptyList a :=
+  match x.tl.reverse with
+  | [] => x
+  | y :: ys => { hd := y, tl := ys ++ [x.hd] }
+
+#eval reverse { hd := 5, tl := [1, 2, 3] }
+
+instance NonEmptyListFunctor : Functor NonEmptyList where
+  map := map
+
+instance NonEmptyListTraversable : Traversable NonEmptyList where
+  traverse := traverse
+
+-- For examples
+section Unsafe
+
+variable [Inhabited a]
+
+protected def fromList! (x: List a): NonEmptyList a := match x with
+| [] => panic "empty list"
+| x :: xs => NonEmptyList.mk x xs
+
+end Unsafe
+
+end NonEmptyList
